Clap/Compiler/Simp.lean
@@ -60,11 +60,58 @@ def SimpSet.union (s₁ s₂ : SimpSet) : SimpSet where
   pos := s₁.pos ++ s₂.pos
   neg := s₁.neg ++ s₂.neg
 
+-- open Sym.Simp in
+-- public def mkSimprocFor (declNames : Array Name) (d : Discharger := dischargeNone) : MetaM Simproc := do
+--   let mut thms : Theorems := {}
+--   for declName in declNames do
+--     thms := thms.insert (← mkTheoremFromDecl declName)
+--   return thms.rewrite d
+
+-- def mkAlternativeSimprocFor (name : Name) : MetaM Sym.Simp.Simproc := do
+--   let thm := Sym.Simp.mkTheoremFromDecl name
+--   _
+
+def simproc? (name : Name) : MetaM (Option ConstantInfo) := do
+  let .some ci := (←getEnv).find? name | throwError m!"Undeclared constant: {name}"
+  return if ci.type.isConstOf `Lean.Meta.Sym.Simp.Simproc
+         then .some ci
+         else .none
+
+def isSimproc (name : Name) : MetaM Bool := return (←simproc? name).isSome
+
+def getSimproc (name : Name) : MetaM Sym.Simp.Simproc := do
+  discard (isSimproc name)
+  let .ok sproc := unsafe (←getEnv).evalConst Sym.Simp.Simproc {} name
+    | throwError m!"Failed to evaluate: {name}"
+  return sproc
+
+def orElse (names : Array Name) : MetaM Sym.Simp.Simproc := do
+  let simprocs ← names.mapM getSimproc
+  return simprocs.foldl (· <|> ·) (fun _ ↦ return .rfl) -- I hope this is the `.continue`...
+
+def andThen (names : Array Name) : MetaM Sym.Simp.Simproc := do
+  let simprocs ← names.mapM getSimproc
+  return simprocs.foldl (· >> ·) (fun _ ↦ return .rfl) -- I hope this is the `.continue`...
+
+instance : Singleton Sym.Simp.Simproc Sym.Simp.Methods where
+  singleton x := {post := x}
+
+instance : Union Sym.Simp.Methods := ⟨
+  fun m₁ m₂ =>
+    {
+      pre := m₁.pre >> m₂.pre
+      post := m₁.post >> m₂.post
+    }
+  ⟩
+
 def SimpSet.toMethods (s : SimpSet) : Sym.SymM Sym.Simp.Methods := do
   unless s.neg.isEmpty do throwError m!"Erasing Sym.simp theorems currently unsupported."
   let (pre, post) := (s.pos.partition fun (_, order) ↦ order matches .Pre).map (·.map Prod.fst) (·.map Prod.fst)
-  let simprocsPre ← Sym.mkSimprocFor pre
-  let simprocsPost ← Sym.mkSimprocFor post
+  let (preSimp, preThm) ← pre.toList.partitionM (liftM ∘ isSimproc)
+  let (postSimp, postThm) ← post.toList.partitionM (liftM ∘ isSimproc)
+  logInfo m!"preThm: {preThm}\npreSimp: {preSimp}\npostThm:{postThm}\npostSimp:{postSimp}"
+  let simprocsPre := (←Sym.mkSimprocFor preThm.toArray) <|> (←andThen preSimp.toArray)
+  let simprocsPost := (← Sym.mkSimprocFor postThm.toArray) <|> (←andThen postSimp.toArray)
   return {
     pre := simprocsPre
     post := simprocsPost
@@ -85,7 +132,7 @@ section
 open Parser Tactic
 
 set_option hygiene false in
-def configStx (singlePass : Bool := false) : Sym.SymM (TSyntax ``optConfig) := do
+def configStx (singlePass : Bool := false) : Sym.Simp.SimpM (TSyntax ``optConfig) := do
   `(optConfig|(
       config := {
         failIfUnchanged := false
@@ -97,7 +144,7 @@ def configStx (singlePass : Bool := false) : Sym.SymM (TSyntax ``optConfig) := d
   where defaultMaxSteps := 10_000_000
 
 def simpSetStx (sets : Array Lemma) :
-  Sym.SymM (Syntax.TSepArray [``simpStar, ``simpErase, ``simpLemma] ",") := do
+  Sym.Simp.SimpM (Syntax.TSepArray [``simpStar, ``simpErase, ``simpLemma] ",") := do
   let arrStx ← sets.mapM fun lemma ↦
     match lemma with
     | .neg name => `(simpErase|-$(mkIdent name):term)
@@ -112,7 +159,7 @@ open API
 
 set_option hygiene false in
 def mkSimp (simpset : SimpSet)
-           (only singlePass : Bool := false) : Sym.SymM (TSyntax `tactic) := do
+           (only singlePass : Bool := false) : Sym.Simp.SimpM (TSyntax `tactic) := do
   let simpsetStx ← simpSetStx simpset.toSimpSet
   if only
   then `(tactic| simp $(←configStx singlePass) only [$[$simpsetStx],*])
@@ -123,14 +170,16 @@ def forceHeartbeats {α : Type} {m : Type → Type} [MonadWithReaderOf Core.Cont
   withTheReader Core.Context ({· with maxHeartbeats := heartBeats * 1000})
 
 set_option hygiene false in
-def simplify (simpset : SimpSet) (e : Expr) (only singlePass : Bool := false) : Sym.SymM Expr := do
-  tryCatchRuntimeEx
-    (forceHeartbeats 300_000 do
+def simplify (simpset : Sym.Simp.Methods) (e : Expr) (only singlePass : Bool := false) : Sym.Simp.SimpM Expr := do
+  -- tryCatchRuntimeEx
+    -- (forceHeartbeats 300_000 do
       lambdaTelescope e fun args body ↦ do
-        let res ← Sym.simp body (←simpset.toMethods) config
+        logInfo m!"Calling Sym.simp on:\n{body}"
+        let res ← Sym.simp body simpset config
+        logInfo m!"Result:\n{res.getResultExpr body}"
         Sym.mkLambdaFVarsS args (res.getResultExpr body)
-    )
-    (fun _ ↦ do throwError s!"Simp Timeout:\n{←PrettyPrinter.ppExpr e}")
+    -- )
+    -- (fun _ ↦ do throwError s!"Simp Timeout:\n{←PrettyPrinter.ppExpr e}")
 
 end Simp
 
